PhysLean/Particles/SuperSymmetry/SU5/ChargeSpectrum/Completions.lean
@@ -34,10 +34,10 @@ variable {𝓩 : Type}
 
 /-- A charge spectrum is complete if it has all types of fields. -/
 def IsComplete (x : ChargeSpectrum 𝓩) : Prop :=
-  x.1.isSome ∧ x.2.1.isSome ∧ x.2.2.1 ≠ ∅ ∧ x.2.2.2 ≠ ∅
+  x.qHd.isSome ∧ x.qHu.isSome ∧ x.Q5 ≠ ∅ ∧ x.Q10 ≠ ∅
 
 instance [DecidableEq 𝓩] (x : ChargeSpectrum 𝓩) : Decidable (IsComplete x) :=
-  inferInstanceAs (Decidable (x.1.isSome ∧ x.2.1.isSome ∧ x.2.2.1 ≠ ∅ ∧ x.2.2.2 ≠ ∅))
+  inferInstanceAs (Decidable (x.qHd.isSome ∧ x.qHu.isSome ∧ x.Q5 ≠ ∅ ∧ x.Q10 ≠ ∅))
 
 @[simp]
 lemma not_isComplete_empty : ¬ IsComplete (∅ : ChargeSpectrum 𝓩) := by
@@ -83,17 +83,36 @@ variable [DecidableEq 𝓩]
   the minimimal charges `y` in `ofFinset S5 S10` which are a super sets of `x` and are
   complete. -/
 def completions (S5 S10 : Finset 𝓩) (x : ChargeSpectrum 𝓩) : Multiset (ChargeSpectrum 𝓩) :=
-  let SqHd := if x.1.isSome then {x.1} else S5.val.map fun y => some y
-  let SqHu := if x.2.1.isSome then {x.2.1} else S5.val.map fun y => some y
-  let SQ5 := if x.2.2.1 ≠ ∅ then {x.2.2.1} else S5.val.map fun y => {y}
-  let SQ10 := if x.2.2.2 ≠ ∅ then {x.2.2.2} else S10.val.map fun y => {y}
-  (SqHd.product (SqHu.product (SQ5.product SQ10)))
+  let SqHd := if x.qHd.isSome then {x.qHd} else S5.val.map fun y => some y
+  let SqHu := if x.qHu.isSome then {x.qHu} else S5.val.map fun y => some y
+  let SQ5 := if x.Q5 ≠ ∅ then {x.Q5} else S5.val.map fun y => {y}
+  let SQ10 := if x.Q10 ≠ ∅ then {x.Q10} else S10.val.map fun y => {y}
+  (SqHd.product (SqHu.product (SQ5.product SQ10))).map (toProd).symm
+
+
+lemma mem_completions_iff {S5 S10 : Finset 𝓩} {x y : ChargeSpectrum 𝓩} :
+    y ∈ completions S5 S10 x ↔
+    y.qHd ∈ (if x.qHd.isSome then {x.qHd} else S5.val.map fun y => some y) ∧
+    y.qHu ∈ (if x.qHu.isSome then {x.qHu} else S5.val.map fun y => some y) ∧
+    y.Q5 ∈ (if x.Q5 ≠ ∅ then {x.Q5} else S5.val.map fun y => {y}) ∧
+    y.Q10 ∈ (if x.Q10 ≠ ∅ then {x.Q10} else S10.val.map fun y => {y}) := by
+  rw [completions]
+  rw [Multiset.mem_map]
+  constructor
+  · rintro ⟨a, h, hy⟩
+    have ha : a = toProd y := by subst hy; simp
+    subst ha
+    simpa [toProd] using h
+  · intro h
+    use toProd y
+    simpa [toProd] using h
 
 lemma completions_nodup (S5 S10 : Finset 𝓩) (x : ChargeSpectrum 𝓩) :
     (completions S5 S10 x).Nodup := by
   simp [completions]
   split_ifs
   all_goals
+    refine Multiset.Nodup.map toProd.symm.injective ?_
     refine Multiset.Nodup.product ?_ (Multiset.Nodup.product ?_ (Multiset.Nodup.product ?_ ?_))
   any_goals exact Multiset.nodup_singleton _
   any_goals exact Finset.nodup_map_iff_injOn.mpr (by simp)
@@ -103,13 +122,13 @@ lemma completions_eq_singleton_of_complete {S5 S10 : Finset 𝓩} (x : ChargeSpe
     completions S5 S10 x = {x} := by
   simp [completions]
   simp [IsComplete] at hcomplete
-  by_cases h1 : x.1.isSome
+  by_cases h1 : x.qHd.isSome
   case' neg => simp_all
-  by_cases h2 : x.2.1.isSome
+  by_cases h2 : x.qHu.isSome
   case' neg => simp_all
-  by_cases h3 : x.2.2.1 ≠ ∅
+  by_cases h3 : x.Q5 ≠ ∅
   case' neg => simp_all
-  by_cases h4 : x.2.2.2 ≠ ∅
+  by_cases h4 : x.Q10 ≠ ∅
   case' neg => simp_all
   simp_all
   rfl
@@ -117,27 +136,25 @@ lemma completions_eq_singleton_of_complete {S5 S10 : Finset 𝓩} (x : ChargeSpe
 @[simp]
 lemma self_mem_completions_iff_isComplete {S5 S10 : Finset 𝓩} (x : ChargeSpectrum 𝓩) :
     x ∈ completions S5 S10 x ↔ IsComplete x := by
-  simp [completions, IsComplete]
-  repeat rw [Multiset.mem_product]
-  by_cases h1 : x.1.isSome
+  simp [mem_completions_iff, IsComplete]
+  by_cases h1 : x.qHd.isSome
+  case neg => simp_all
+  by_cases h2 : x.qHu.isSome
   case' neg => simp_all
-  by_cases h2 : x.2.1.isSome
+  by_cases h3 : x.Q5 ≠ ∅
   case' neg => simp_all
-  by_cases h3 : x.2.2.1 ≠ ∅
+  by_cases h4 : x.Q10 ≠ ∅
   case' neg => simp_all
-  by_cases h4 : x.2.2.2 ≠ ∅
-  case' neg => simp_all
+
   simp_all
 
 lemma mem_completions_isComplete {S5 S10 : Finset 𝓩} {x y : ChargeSpectrum 𝓩}
     (hx : y ∈ completions S5 S10 x) : IsComplete y := by
   match y with
-  | (qHd, qHu, Q5, Q10) =>
-  simp [completions] at hx
-  repeat rw [Multiset.mem_product] at hx
-  simp at hx
+  | ⟨qHd, qHu, Q5, Q10⟩ =>
+  simp [mem_completions_iff] at hx
   match x with
-  | (x1, x2, x3, x4) =>
+  | ⟨x1, x2, x3, x4⟩ =>
   simp_all
   rw [IsComplete]
   refine ⟨?_, ?_, ?_, ?_⟩
@@ -168,21 +185,20 @@ lemma mem_completions_isComplete {S5 S10 : Finset 𝓩} {x y : ChargeSpectrum �
 
 lemma self_subset_mem_completions (S5 S10 : Finset 𝓩) (x y : ChargeSpectrum 𝓩)
     (hy : y ∈ completions S5 S10 x) : x ⊆ y := by
-  simp [completions] at hy
-  repeat rw [Multiset.mem_product] at hy
+  simp [mem_completions_iff] at hy
   rw [Subset]
   dsimp [hasSubset]
   refine ⟨?_, ?_, ?_, ?_⟩
-  · by_cases h : x.1.isSome
+  · by_cases h : x.qHd.isSome
     · simp_all
     · simp_all
-  · by_cases h : x.2.1.isSome
+  · by_cases h : x.qHu.isSome
     · simp_all
     · simp_all
-  · by_cases h : x.2.2.1 ≠ ∅
+  · by_cases h : x.Q5 ≠ ∅
     · simp_all
     · simp_all
-  · by_cases h : x.2.2.2 ≠ ∅
+  · by_cases h : x.Q10 ≠ ∅
     · simp_all
     · simp_all
 
@@ -195,7 +211,7 @@ lemma exist_completions_subset_of_complete (S5 S10 : Finset 𝓩) (x y : ChargeS
   rw [Subset] at hsubset
   dsimp [hasSubset] at hsubset
   match x, y with
-  | (x1, x2, x3, x4), (y1, y2, y3, y4) =>
+  | ⟨x1, x2, x3, x4⟩, ⟨y1, y2, y3, y4⟩ =>
   simp [IsComplete] at hycomplete
   rw [Option.isSome_iff_exists, Option.isSome_iff_exists] at hycomplete
   obtain ⟨y1, rfl⟩ := hycomplete.1
@@ -204,11 +220,12 @@ lemma exist_completions_subset_of_complete (S5 S10 : Finset 𝓩) (x y : ChargeS
   simp at hycomplete
   obtain ⟨z3, hz3⟩ := hycomplete.1
   obtain ⟨z4, hz4⟩ := hycomplete.2
+  simp [mem_ofFinset_iff] at hy
   have hz3Mem : z3 ∈ S5 := by
-    apply mem_ofFinset_Q5_subset S5 S10 hy
+    apply hy.2.2.1
     simp_all
   have hz4Mem : z4 ∈ S10 := by
-    apply mem_ofFinset_Q10_subset S5 S10 hy
+    apply hy.2.2.2
     simp_all
   have hy1' : some y1 ∈ if x1.isSome = true then {x1} else
       Multiset.map (fun y => some y) S5.val := by
@@ -218,7 +235,6 @@ lemma exist_completions_subset_of_complete (S5 S10 : Finset 𝓩) (x y : ChargeS
       obtain ⟨a, rfl⟩ := h1
       simp_all
     · simp_all
-      exact qHd_mem_ofFinset S5 S10 y1 (some y2, y3, y4) hy
   have hy2' : some y2 ∈ if x2.isSome = true then {x2} else
       Multiset.map (fun y => some y) S5.val := by
     by_cases h2 : x2.isSome
@@ -227,46 +243,37 @@ lemma exist_completions_subset_of_complete (S5 S10 : Finset 𝓩) (x y : ChargeS
       obtain ⟨a, rfl⟩ := h2
       simp_all
     · simp_all
-      exact qHu_mem_ofFinset S5 S10 y2 (some y1) (y3, y4) hy
   simp_all
   by_cases h3 : x3 ≠ ∅
   · by_cases h4 : x4 ≠ ∅
-    · use (y1, y2, x3, x4)
+    · use ⟨y1, y2, x3, x4⟩
       constructor
-      · simp_all [completions]
-        repeat rw [Multiset.mem_product]
-        simp_all
+      · simp_all [mem_completions_iff]
       · rw [Subset]
         dsimp [hasSubset]
         simp_all
     · simp at h4
       subst h4
-      use (y1, y2, x3, {z4})
+      use ⟨y1, y2, x3, {z4}⟩
       constructor
-      · simp [completions]
-        repeat rw [Multiset.mem_product]
-        simp_all
+      · simp_all [mem_completions_iff]
       · rw [Subset]
         dsimp [hasSubset]
         simp_all
   · simp at h3
     subst h3
     by_cases h4 : x4 ≠ ∅
-    · use (y1, y2, {z3}, x4)
+    · use ⟨y1, y2, {z3}, x4⟩
       constructor
-      · simp [completions]
-        repeat rw [Multiset.mem_product]
-        simp_all
+      · simp_all [mem_completions_iff]
       · rw [Subset]
         dsimp [hasSubset]
         simp_all
     · simp at h4
       subst h4
-      use (y1, y2, {z3}, {z4})
+      use ⟨y1, y2, {z3}, {z4}⟩
       constructor
-      · simp [completions]
-        repeat rw [Multiset.mem_product]
-        simp_all
+      · simp_all [mem_completions_iff]
       · rw [Subset]
         dsimp [hasSubset]
         simp_all
@@ -281,7 +288,7 @@ lemma exist_completions_subset_of_complete (S5 S10 : Finset 𝓩) (x y : ChargeS
   `minimallyAllowsTermsOfFinset S5 S10 .topYukawa`. -/
 def completionsTopYukawa (S5 : Finset 𝓩) (x : ChargeSpectrum 𝓩) :
     Multiset (ChargeSpectrum 𝓩) :=
-  (S5.val.product S5.val).map fun (qHd, q5) => (qHd, x.2.1, {q5}, x.2.2.2)
+  (S5.val.product S5.val).map fun (qHd, q5) => ⟨qHd, x.qHu, {q5}, x.Q10⟩
 
 omit [DecidableEq 𝓩] in
 lemma completionsTopYukawa_nodup {S5 : Finset 𝓩} (x : ChargeSpectrum 𝓩) :
@@ -310,8 +317,7 @@ lemma completions_eq_completionsTopYukawa_of_mem_minimallyAllowsTermsOfFinset [A
     simp at hcard
   simp [Q10_neq_zero]
   match a with
-  | (xqHd, xqHu, xQ5, xQ10) =>
-  repeat rw [Multiset.mem_product]
+  | ⟨xqHd, xqHu, xQ5, xQ10⟩ =>
   simp [eq_iff]
   aesop
 
